FCB correct (#4)

theories/Example/Lambda.v
@@ -1,26 +1,27 @@
-From Nominal Require Import Nominal Fresh Alpha NameAbstraction.
-From Nominal.Instances Require Import SupportedFunctions Name Prod Perm.
+From Coq Require Import Lists.List.
+From Nominal Require Export Nominal Fresh NameAbstraction FreshnessTheorem.
+From Nominal.Instances Require Export SupportedFunctions Name Prod Perm.
 
-Inductive Term : Set :=
-| Var: Name → Term
-| App: Term → Term → Term
-| Lam: Name → Term → Term.
+Inductive Λ : Set :=
+| Var: Name → Λ
+| App: Λ → Λ → Λ
+| Lam: Name → Λ → Λ.
 
-Fixpoint atms (t: Term) : NameSet :=
+Fixpoint atms (t: Λ) : NameSet :=
   match t with
   | Var a => {[ a ]}
   | App t1 t2 => (atms t1) ∪ (atms t2)
   | Lam a t => {[ a ]} ∪ (atms t)
   end.
 
-Fixpoint term_action (p: Perm) (t: Term): Term :=
+Fixpoint term_action (p: Perm) (t: Λ): Λ :=
   match t with
   | Var a => Var (p • a)
   | App m n => App (term_action p m) (term_action p n)
   | Lam a m => Lam (p • a) (term_action p m)
   end.
 
-Instance TermAction: PermAction Term := term_action.
+Instance TermAction: PermAction Λ := term_action.
 
 Lemma term_perm_var p a : p • (Var a) = Var (p • a).
 Proof. unfold action; simpl; reflexivity. Qed.
@@ -45,7 +46,7 @@ Proof.
   - do 2 rewrite term_perm_abs; f_equal; auto.
 Qed.
 
-Lemma term_perm_id (t : Term): ɛ•t = t.
+Lemma term_perm_id (t : Λ): ɛ•t = t.
 Proof.
   induction t.
   - rewrite term_perm_var; auto.
@@ -53,7 +54,7 @@ Proof.
   - rewrite term_perm_abs; rewrite IHt; auto.
 Qed.
 
-Lemma term_perm_compat p q (t : Term): p•(q•t) = (q + p)•t.
+Lemma term_perm_compat p q (t : Λ): p•(q•t) = (q + p)•t.
 Proof.
   induction t.
   - repeat rewrite term_perm_var; f_equal; apply gact_compat.
@@ -61,10 +62,10 @@ Proof.
   - repeat rewrite term_perm_abs; f_equal; [apply gact_compat |]; auto.
 Qed. 
 
-Lemma term_perm_swap_distr a b (p : Perm) (x: Term) : p•⟨a,b⟩•x = ⟨p•a, p•b⟩•p•x.
+Lemma term_perm_swap_distr a b (p : Perm) (x: Λ) : p•⟨a,b⟩•x = ⟨p•a, p•b⟩•p•x.
 Proof. rewrite 2term_perm_compat; apply term_perm_proper; auto; apply perm_comm_distr. Qed.
 
-Lemma term_action_neither (a b: Name) (t: Term) : 
+Lemma term_action_neither (a b: Name) (t: Λ) : 
   a ∉ atms t → b ∉ atms t → ⟨a,b⟩•t = t.
 Proof.
   induction t; intros.
@@ -73,7 +74,7 @@ Proof.
   - rewrite term_perm_abs,name_action_neither,IHt; simpl in *; set_solver.
 Qed.
 
-Lemma term_action_equal (a : Name) (t: Term) : 
+Lemma term_action_equal (a : Name) (t: Λ) : 
   ⟨a,a⟩•t = t.
 Proof.
   induction t; intros.
@@ -82,48 +83,41 @@ Proof.
   - rewrite term_perm_abs,!perm_equiv_neutral,IHt; reflexivity.
 Qed.
 
-Lemma term_action_inv (a b: Name) (t: Term) : 
+Lemma term_action_inv (a b: Name) (t: Λ) : 
   ⟨a,b⟩•t = -⟨a,b⟩•t.
-Proof. Admitted.
-  (* induction t; intros.
-  - rewrite term_perm_var,perm_equiv_neutral; f_equal.
+Proof.
+  induction t; intros.
+  - rewrite !term_perm_var; f_equal.
   - rewrite term_perm_app,IHt1,IHt2; reflexivity.
-  - rewrite term_perm_abs,!perm_equiv_neutral,IHt; reflexivity.
-Qed. *)
+  - rewrite !term_perm_abs; f_equal.
+Qed.
 
-Lemma term_action_swap (a b: Name) (t: Term) : 
+Lemma term_action_swap (a b: Name) (t: Λ) : 
   ⟨a,b⟩•t = ⟨b,a⟩•t.
-Proof. Admitted.
-  (* induction t; intros.
-  - rewrite term_perm_var,perm_equiv_neutral; f_equal.
+Proof.
+  induction t; intros.
+  - rewrite !term_perm_var; f_equal; rewrite swap_perm; reflexivity.
   - rewrite term_perm_app,IHt1,IHt2; reflexivity.
-  - rewrite term_perm_abs,!perm_equiv_neutral,IHt; reflexivity.
-Qed. *)
+  - rewrite !term_perm_abs; f_equal; [rewrite swap_perm |]; auto.
+Qed.
 
 End PermTerm.
 
-(* Inductive aeq: Term → Term → Prop :=
+(* Inductive aeq: Λ → Λ → Prop :=
 | AeqVar: ∀ a, aeq (Var a) (Var a)
 | AeqApp: ∀ m m' n n', aeq m m' → aeq n n' → aeq (App m n) (App m' n')
 | AeqAbs: ∀ a b m n, 
   (∀ c, c ≠ a → c ≠ b → c ∉ atms m → c ∉ atms n → 
     aeq (⟨a,c⟩•m) (⟨b,c⟩•n)) → aeq (Lam a m) (Lam b n). *)
 
-Inductive aeqCof: Term → Term → Prop :=
-| AeqVarC: ∀ a, aeqCof (Var a) (Var a)
-| AeqAppC: ∀ m m' n n', aeqCof m m' → aeqCof n n' → aeqCof (App m n) (App m' n')
-| AeqAbsC: ∀ (L : NameSet) a b m n, 
-  (∀ c, c ∉ L → aeqCof (⟨a,c⟩•m) (⟨b,c⟩•n)) → aeqCof (Lam a m) (Lam b n).
+Reserved Notation "a ≡α b" (at level 61).
+Inductive aeqCof: Λ → Λ → Prop :=
+| AeqVarC: ∀ a, (Var a) ≡α (Var a)
+| AeqAppC: ∀ m m' n n', m ≡α m' → n ≡α n' → (App m n) ≡α (App m' n')
+| AeqAbsC: ∀ (L : NameSet) a b m n, (∀ c, c ∉ L → (⟨a,c⟩•m) ≡α (⟨b,c⟩•n)) → (Lam a m) ≡α (Lam b n)
+where "a ≡α b" := (aeqCof a b).
 
-(* Lemma term_perm_alpha_ p m n: aeq m n → aeq (p • m) (p • n).
-Proof. 
-  induction 1.
-  - rewrite term_perm_var; constructor.
-  - repeat rewrite term_perm_app; constructor; auto.
-  - repeat rewrite term_perm_abs; constructor; intros. *)
-
-
-Lemma term_perm_alpha p m n: aeqCof m n → aeqCof (p • m) (p • n).
+Lemma term_perm_alpha p m n: m ≡α n → (p • m) ≡α (p • n).
 Proof. 
   induction 1.
   - rewrite term_perm_var; constructor.
@@ -134,28 +128,32 @@ Proof.
       do 2 rewrite <-term_perm_swap_distr; apply H0; set_solver.
 Qed.
 
-(* Theorem aeqs_equal m n: aeq m n <-> aeqCof m n.
+(* Lemma term_perm_alpha_ a b m n: aeq m n → aeq (⟨a,b⟩•m) (⟨a,b⟩•n).
+Proof. Admitted.
+
+Theorem aeqs_equal m n: aeq m n ↔ m ≡α n.
 Proof.
-  split; induction 1.
-  - constructor.
-  - constructor; auto.
-  - apply AeqAbsC with (L := ({[a;b]} ∪ (atms m) ∪ (atms n))); intros c Hc;
-    apply H0; set_solver.
-  - constructor.
-  - constructor; auto.
-  - constructor; intros; destruct (exist_fresh ({[a;b;c]} ∪ (atms m) ∪ (atms n) ∪ L)) as [d Hd].
-    assert (HH: d ∉ L). { set_solver. } specialize (H0 d HH).
-    apply (term_perm_alpha_ (⟨c,d⟩)) in H0. 
-    rewrite 2(term_perm_swap_distr _ _ ⟨c,d⟩) in H0.
-    rewrite name_action_right in H0.
-    rewrite 2name_action_neither in H0; [| set_solver | set_solver | set_solver | set_solver].
-    assert (HH2 : ⟨ c, d ⟩ • m = m). { apply term_action_neither; set_solver. }
-    assert (HH3 : ⟨ c, d ⟩ • n = n). { apply term_action_neither; set_solver. }
-    rewrite HH2,HH3 in H0; auto.
+  split; intros H.
+  - induction H.
+    + constructor.
+    + constructor; auto. 
+    + apply AeqAbsC with (L := ({[a;b]} ∪ (atms m) ∪ (atms n))); intros c Hc.
+      apply H0; set_solver.
+  - induction H.
+    + constructor.
+    + constructor; auto.
+    + constructor; intros. destruct (exist_fresh ({[a;b;c]} ∪ (atms m) ∪ (atms n) ∪ L)) as [d Hd].
+      assert (HH: d ∉ L). { set_solver. } specialize (H0 d HH). Admitted.
+      (* apply term_perm_alpha_ with (p := ⟨c,d⟩) in H0.
+      rewrite 2(term_perm_swap_distr _ _ ⟨c,d⟩) in H0.
+      rewrite name_action_right in H0.
+      rewrite 2name_action_neither in H0; [| set_solver | set_solver | set_solver | set_solver].
+      assert (HH2 : ⟨ c, d ⟩ • m = m). { apply term_action_neither; set_solver. }
+      assert (HH3 : ⟨ c, d ⟩ • n = n). { apply term_action_neither; set_solver. }
+      rewrite HH2,HH3 in H0; auto. *)
 Qed. *)
     
 Instance AeqCofRef: Reflexive aeqCof.
-
 Proof.
   intros t; induction t.
   - constructor.
@@ -183,9 +181,9 @@ Qed.
 Instance AeqCofEquiv : Equivalence aeqCof.
 Proof. split; typeclasses eauto. Qed.
 
-Instance TermEquiv : Equiv Term := aeqCof.
+Instance TermEquiv : Equiv Λ := aeqCof.
 
-Instance TermPermT : PermT Term.
+Instance TermPermT : PermT Λ.
 Proof.
   split.
   - typeclasses eauto.
@@ -200,16 +198,16 @@ Proof.
   - intros; rewrite term_perm_compat; reflexivity.
 Qed. 
 
-Fixpoint fv (t: Term): NameSet :=
+Fixpoint fv (t: Λ): NameSet :=
   match t with
   | Var a => {[ a ]}
   | App m n => (fv m) ∪ (fv n)
   | Lam a m => (fv m) ∖ {[ a ]}
   end.
 
-Instance TermSupport : Support Term := fv.
+Instance TermSupport : Support Λ := fv.
 
-Instance TermNominal : Nominal Term.
+Instance TermNominal : Nominal Λ.
 Proof.
   split.
   - exact TermPermT.
@@ -233,311 +231,19 @@ Proof.
         -- apply elem_of_singleton in H0,H; subst; congruence.
 Qed.
 
-(* Definition term_rect_general := fun (P : Term → Type)
-  (fvar : ∀ a : Name, P (Var a))
-  (fapp : ∀ t1: Term, P t1 → ∀ t2: Term, P t2 → P (App t1 t2))
-  (flam : ∀ a : Name, ∀ t: Term, P t → P (Lam (a,t))) =>
-  fix F (t: Term) : P t :=
-    match t as t' return (P t') with
-    | Var a => fvar a
-    | App t1 t2 => fapp t1 (F t1) t2 (F t2)
-    | Lam (a, t) => flam a t (F t)
-    end. *)
+Instance term_rewrite_var: Proper (eq ==> equiv) (Var).
+Proof. repeat intro; rewrite H; reflexivity. Qed.
 
-(* Definition term_rec_general (P : Term → Set) := term_rect_general P.
-Definition term_ind_general (P : Term → Prop) := term_rect_general P. *)
+Instance term_rewrite_app: Proper (equiv ==> equiv ==> equiv) (App).
+Proof. repeat intro; apply AeqAppC; auto. Qed.
 
-(* Fixpoint atm (t: Term) : NameSet.
-Proof.
-  apply term_rec_general.
-  - exact (λ a, {[ a ]}).
-  - exact (λ _ fm _ fn, fm ∪ fn).
-  - exact (λ a _ fm, {[ a ]} ∪ fm).
-  - exact t.
-Defined. *)
-
-(* 
-Definition subst_name (c a b: Name): Name :=
-  if Atom.dec c b then a else c.
-
-Lemma subst_neq (a b c: Name) : c ≠ b → subst_name c a b = c.
-Proof. intros; unfold subst_name; destruct Atom.dec; subst; [congruence | reflexivity]. Qed.
-
-Lemma subst_eq (a b c: Name) : c = b → subst_name c a b = a.
-Proof. intros; unfold subst_name; destruct Atom.dec; subst; [reflexivity | congruence]. Qed.
-
-Fixpoint subst (t: Term) (a b: Name) : Term :=
-  match t with
-  | Var c => Var (subst_name c a b)
-  | App t1 t2 => App (subst t1 a b) (subst t2 a b)
-  | Lam (c,t) => Lam ((subst_name c a b), (subst t a b))
-  end.
-
-Lemma subst_notin_atm t a b: b ∉ atm t → subst t a b = t.
-Proof. induction t using term_ind_general; intros; simpl in *.
-  - rewrite subst_neq; [reflexivity | set_solver].
-  - rewrite IHt1, IHt2; set_solver.
-  - rewrite IHt.
-    + rewrite subst_neq; [reflexivity | set_solver].
-    + set_solver.  
-Qed.
-
-Lemma subst_equal m a: subst m a a = m.
-Proof. 
-  induction m using term_ind_general; intros; simpl in *. 
-  - destruct (decide (a0 = a)); [rewrite subst_eq | rewrite subst_neq]; subst; auto.
-  - rewrite IHm1, IHm2; reflexivity.
-  - destruct (decide (a0 = a)); [rewrite subst_eq | rewrite subst_neq]; 
-      subst; try rewrite IHm; auto.
-Qed.
-
-Lemma subst_var a b c : a = c → subst (Var a) b c = Var b.
-Proof. intros; simpl; rewrite subst_eq; auto. Qed.
-
-Lemma subst_var_neq a b c : a ≠ c → subst (Var a) b c = Var a.
-Proof. intros; simpl; rewrite subst_neq; auto. Qed.
-
-Inductive aeq: Term → Term → Prop :=
-| AeqVar: ∀ a, aeq (Var a) (Var a)
-| AeqApp: ∀ m n m' n', aeq m m' → aeq n n' → aeq (App m n) (App m' n')
-| AeqAbs: ∀ (a b: Name) (m n: Term), 
-    (∀ c, c ≠ a → c ≠ b → c ∉ atm m → c ∉ atm n → aeq (subst m c a) (subst n c b)) → 
-    aeq (Lam (a,m)) (Lam (b,n)).
-
-Lemma aeq_subst_notin: ∀ m n a c, 
-  c ∉ atm m → c ∉ atm n → aeq m n → aeq (subst m a c) (subst n a c).
-Proof. intros; do 2 (try rewrite subst_notin_atm); auto. Qed.
-
-Lemma aeq_subst: ∀ m n a c, 
-  aeq m n → aeq (subst m a c) (subst n a c).
-Proof.
-  intros; inversion H.
-  - destruct (decide (a0 = c)); [rewrite subst_var | rewrite subst_var_neq]; auto; constructor.
-  - admit.
-  - simpl; constructor; intro w; intros.
-    destruct (decide (a0 = b)); subst.
-    +    
-   destruct (decide (a0 = c)), (decide (b = c)); subst.
-    + rewrite subst_eq; auto. specialize (H0 a).
-      
-     apply H0.
-
-Instance subst_proper: Proper (aeq ==> eq ==> eq ==> aeq) subst.
-Proof. repeat intro; subst. apply aeq_subst; auto.
-
-#[export] Instance: Equiv Term := aeq.
-#[export] Instance: Reflexive aeq.
-Proof.
-  intro x; induction x using term_ind_general.
-  - constructor.
-  - constructor; auto.
-  - destruct (exist_fresh ({[a]} ∪ (atm1 x))) as [c Hc]; apply AeqAbs with (c := c).
-    + split; set_solver.
-    + split; set_solver. 
-    + apply aeq_subst; set_solver.
-Qed.
-
-#[export] Instance: Symmetric aeq.
-Proof.
-  repeat intro; induction H.
-  - constructor.
-  - constructor; auto.
-  - econstructor; [destruct H; split; eauto | intuition | auto].
-Qed.
-
-#[export] Instance: Transitive aeq.
-Proof. Admitted.
-
-#[export] Instance: Equivalence aeq.
-Proof. split; typeclasses eauto. Qed.
-
-#[export] Instance: Equiv Term := aeq. *)
-
-(* Fixpoint taction (p: Perm) (t: Term): Term :=
-  match t with
-  | Var a => Var (p • a)
-  | App m n => App (taction p m) (taction p n)
-  | Lam (a,m) => Lam ((p • a), (taction p m))
-  end. *)
-
-(* #[export] Instance: PermT Term.
-Proof.
-  split.
-  - typeclasses eauto.
-  - intros p q PEq m n TEq; (* rewrite PEq *)
-    unfold equiv, perm_equiv, Equiv_instance_1 in *.
-    unfold action, PermAction_instance_0 in *.
-    induction TEq; simpl.
-    + rewrite PEq. reflexivity.
-    + constructor; auto.
-    + econstructor.
-      * (* facil, basta pegar um C diferente *) admit.
-      * (* facil, basta pegar um C diferente *) admit.
-      * (* algume lema que relacione action e subst. *) admit.
-  - intro t; induction t using term_ind_general; unfold action, PermAction_instance_0 in *;
-    simpl.
-    + rewrite gact_id; reflexivity.
-    + constructor; [rewrite IHt1 | rewrite IHt2]; reflexivity.
-    + rewrite gact_id. econstructor.
-      * admit.
-      * admit.
-      * unfold action, PermAction_instance_0 in *; simpl; rewrite IHt; reflexivity.
-  - intros p q t; induction t using term_ind_general; unfold action, PermAction_instance_0 in *;
-    simpl.
-    + rewrite gact_compat; reflexivity.
-    + constructor; auto.
-    + rewrite gact_compat; econstructor.
-      * admit.
-      * admit.
-      * rewrite IHt; reflexivity.      
-Admitted. *)
-
-(* #[export] Instance TermNominal: Nominal Term.
-Proof. split.
-    - typeclasses eauto.
-    - intros t a b Sa Sb;
-      unfold action, TermAction, support, TermSupport,
-                equiv, TermEquiv in *.
-      induction t; simpl in *.
-      + rewrite support_spec; auto; reflexivity.
-      + constructor; [apply IHt1 | apply IHt2]; set_solver. 
-      + admit.
-Admitted. *)
-      (* + apply not_elem_of_difference in Sa, Sb; destruct Sa, Sb.
-        * econstructor; admit. (* a ∉ fv t ∧ b ∉ fv t*)
-        * econstructor; admit. (* a ∉ fv t ∧ b = a0 *)
-        * econstructor; admit. (* a = a0 ∧ b ∉ fv t*)
-        * econstructor; admit. a = a0 ∧ b = a0 *)
-
-Section FreshnessTheorem.
-  Context `{Nominal X} (h: Name →ₛ X).
-  
-  Definition freshF : X := h (fresh (support h)).
-
-  Lemma freshness_theorem_some_any :
-    (∃ a, a # h ∧ a # (h a)) ↔ (∀ a, a # h → a # (h a)).
-  Proof.
-    split; intros HH.
-    - intros a AH; destruct HH as [b [BH1 BH2]]; destruct (decide (a = b)).
-      + subst; assumption.
-      + apply (fresh_equivariant ⟨a,b⟩) in BH2; 
-        rewrite perm_swap_right,fun_equivar,perm_swap_right,fresh_fixpoint in BH2; assumption.
-    - new c fresh h; exists c; split.
-      + apply support_fresh; assumption.
-      + apply HH, support_fresh; assumption.
-  Qed.
-
-  Theorem freshness_theorem (Haf: ∃ a, a # h ∧ a # (h a)) :
-    ∀ a, a # h → (h a) ≡ freshF.
-  Proof.
-    intros a AH; unfold freshF; set (a' := fresh _); destruct (decide (a = a')); subst; try reflexivity.
-    rewrite <-(fresh_fixpoint a a' (h a')), fun_equivar,perm_swap_right,fresh_fixpoint.
-      + reflexivity.
-      + assumption.
-      + apply fresh_support_fresh.
-      + apply fresh_fun_supp; [| apply name_neq_fresh_iff]; assumption.
-      + apply freshness_theorem_some_any; [| apply fresh_support_fresh]; assumption.
-  Qed.
-
-  Corollary freshness_theorem2 :
-    ∀ a b, (∃ (c: Name), c ∉ support h ∧ c # (h c)) → a # h → b # h → h a ≡ h b.
-  Proof. 
-    intros; rewrite !freshness_theorem; try reflexivity; try assumption;
-    destruct H1 as [x ?]; exists x; split; try (apply support_fresh; tauto); tauto.
-  Qed.
-
-End FreshnessTheorem.
-
-(* Definition FCB `{Nominal X, Nominal Y} (f: X →ₛ Y) :=
-  { a | a ∉ (support f) ∧ (∀ x: X, a # (f x)) }.
-
-Theorem freshness_theorem `{Nominal X} (f: Name →ₛ X): 
-  ∀ a b, (∃ (c: Name), c ∉ support f ∧ c # (f c)) → 
-  a # f → b # f → f a ≡ f b.
-Proof. 
-  intros ? ? [c []] ? ?. 
-  rewrite <-(fresh_fixpoint c a f) at 1; auto; try (apply support_fresh; assumption).
-  rewrite <-(fresh_fixpoint c b f) at 2; auto; try (apply support_fresh; assumption).
-  unfold action, fun_supp_act; simpl; rewrite <-!perm_inv, !name_action_right.
-  destruct (decide (c = a)), (decide (c = b)); subst; try rewrite perm_action_equal.
-  - reflexivity.
-  - rewrite fresh_fixpoint; [reflexivity | assumption | idtac].
-    apply fresh_fun_supp; auto; apply name_neq_fresh_iff, not_eq_sym; assumption.
-  - rewrite fresh_fixpoint; [reflexivity | assumption | idtac].
-    apply fresh_fun_supp; auto; apply name_neq_fresh_iff, not_eq_sym; assumption.
-  - rewrite !fresh_fixpoint; try reflexivity; try assumption;
-      apply fresh_fun_supp; auto; apply name_neq_fresh_iff, not_eq_sym; assumption.
-Qed. *)
-
-
-(* all this lemmas can be rewritten using a much more general lemma *)
-
-(* Lemma perm_distr_1 (a b w z: Name) (p: Perm):
-  w ≠ a → w ≠ b → z ≠ a → z ≠ b →
-  ⟨a,b⟩ + (⟨w, z⟩•p) ≡ (⟨w, z⟩•⟨a,b⟩) + (⟨w,z⟩•p).
-Proof.
-  intros; rewrite <-(fresh_fixpoint w z (⟨ a, b ⟩)) at 1; auto;
-  apply support_fresh; set_solver.
-Qed.
-
-Lemma perm_distr_2 (a b w z: Name) (p: Perm):
-  (⟨w,z⟩•⟨a,b⟩) + (⟨w,z⟩•p) ≡ ⟨w,z⟩•(⟨a,b⟩ + p).
-Proof.
-  unfold action, PermActionPerm; rewrite <-perm_inv, !grp_assoc.
-  assert (H: ⟨w,z⟩+⟨a,b⟩+⟨w,z⟩+⟨w,z⟩+p+⟨w,z⟩ ≡ ⟨w,z⟩+⟨a,b⟩+(⟨w,z⟩+⟨w,z⟩)+p+⟨w,z⟩). {
-    rewrite !grp_assoc; reflexivity.
-  }
-  rewrite H, perm_duplicate; clear H.
-  assert (H: ⟨w,z⟩+⟨a,b⟩+ɛ+p+⟨w,z⟩ ≡ ⟨w,z⟩+⟨a,b⟩+(ɛ+(p+⟨w,z⟩))). {
-    rewrite !grp_assoc; reflexivity.
-  }
-  rewrite H, grp_left_id, !grp_assoc; reflexivity.
-Qed.
-
-Lemma perm_distr_3 (a b w z: Name) (p: Perm):
-  w ∉ perm_dom p → z ∉ perm_dom p → w ≠ a → z ≠ a →
-  ⟨w,z⟩•⟨a,b⟩+p ≡ ⟨a,⟨w,z⟩•b⟩+p.
-Proof.
-  intros Pw Pz ? ?; rewrite perm_distr; do 2 unfold action at 1; unfold perm_action.
-  assert (HH1: -⟨w,z⟩+(⟨a,b⟩+⟨w,z⟩)+(-⟨w,z⟩+(p+⟨w,z⟩)) ≡ (⟨a,⟨w,z⟩•b⟩+p)). {
-    rewrite <-perm_inv, !grp_assoc.
-    assert (HH2: ⟨w,z⟩+⟨a,b⟩+⟨w,z⟩+⟨w,z⟩+p+⟨w,z⟩ ≡ ⟨w,z⟩+⟨a,b⟩+p+⟨w,z⟩). {
-      assert (HH3: ⟨w,z⟩+⟨a,b⟩+⟨w,z⟩+⟨w,z⟩+p+⟨w,z⟩ ≡ ⟨w,z⟩+⟨a,b⟩+(⟨w,z⟩+⟨w,z⟩)+p+⟨w,z⟩). {
-      rewrite !grp_assoc; reflexivity.
-      } rewrite HH3, perm_duplicate; clear HH3.
-      assert (HH3: ⟨w,z⟩+⟨a,b⟩+ɛ+p+⟨w,z⟩ ≡ ⟨w,z⟩+⟨a,b⟩+(ɛ+(p+⟨w,z⟩))). {
-        rewrite !grp_assoc; reflexivity.
-      } rewrite HH3, grp_left_id, !grp_assoc; reflexivity.
-    } rewrite HH2; clear HH2; pose proof (perm_notin_dom_comm w z p Pw Pz) as HH.
-    assert (HH2: ⟨w,z⟩+⟨a,b⟩+p+⟨w,z⟩ ≡ ⟨w,z⟩+⟨a,b⟩+⟨w,z⟩+p). {
-      assert (HH3: ⟨w,z⟩+⟨a,b⟩+p+⟨w,z⟩ ≡ ⟨w,z⟩+⟨a,b⟩+(p+⟨w,z⟩)). {
-        rewrite !grp_assoc; reflexivity.
-      } rewrite HH3, <-HH, grp_assoc; reflexivity.
-    } rewrite HH2; clear HH2.
-    pose proof (perm_comm_distr a b ⟨ w, z ⟩) as H2; rewrite perm_swap_neither in H2;
-    try (apply not_eq_sym; auto).
-    assert (HH2: ⟨w,z⟩+⟨a,b⟩+⟨w,z⟩+p ≡ ⟨w,z⟩+(⟨a,b⟩+⟨w,z⟩)+p). {
-      rewrite !grp_assoc; reflexivity.
-    } rewrite HH2, H2, !grp_assoc, perm_duplicate, grp_left_id; 
-    unfold action; simpl; reflexivity.
-  }
-  assert (HH2: (-⟨w,z⟩+(⟨a,b⟩+⟨w,z⟩)+(-⟨w,z⟩+(p+⟨w,z⟩))) ≡ (⟨a,⟨w,z⟩•b⟩+p)). {
-    rewrite HH1; reflexivity.
-  } rewrite HH2; reflexivity.
-Qed. *)
+Instance term_rewrite_lam: Proper (eq ==> equiv ==> equiv) (Lam).
+Proof. repeat intro; apply AeqAbsC with (L := ∅); intros; rewrite H; apply perm_inj; assumption. Qed.
 
 Tactic Notation "eabstract" tactic3(tac) :=
 let G := match goal with |- ?G => G end in
 let pf := constr:(ltac:(tac) : G) in
 abstract exact_no_check pf.
-
-(* Lemma perm_swap_subst_name a b c: 
-  b ≠ c → subst_name c b a = perm_swap ⟨ a, b ⟩ c.
-Proof.
-  intros; unfold subst_name; simpl;
-  destruct (_ =n _); repeat destruct (decide (_ = _)); subst; auto;
-  try congruence.
-Qed. *)
 
 Lemma action_var a b c: ⟨a,b⟩ • Var c = Var (⟨a,b⟩•c).
 Proof. unfold action; simpl; reflexivity. Qed.
@@ -557,56 +263,112 @@ Proof. unfold action; simpl; reflexivity. Qed.
 Lemma perm_lam p a t: p • (Lam a t) = Lam (p•a) (p•t).
 Proof. unfold action; simpl; reflexivity. Qed.
 
-(* Lemma action_subst a b t: b ∉ atm1 t → (subst t b a) = ⟨a, b⟩ • t.
-Proof.
-  intros; induction t using term_ind_general.
-  - unfold action; simpl; unfold action, name_action; rewrite perm_swap_subst_name;
-    auto; set_solver.
-  - simpl in *; rewrite action_app; f_equal; [apply IHt1 | apply IHt2]; set_solver.
-  - simpl in *; rewrite action_lam; do 2 f_equal; [apply perm_swap_subst_name | apply IHt]; set_solver.
-Qed. *)
+Lemma var_fresh (a b: Name): a # Var b → a ≠ b.
+Proof. 
+   intros; apply some_any_iff in H; unfold freshP_a in H; 
+   destruct (exist_fresh (support a ∪ support b ∪ support (Var b))) as [w Hw];
+   specialize (H w ltac:(set_solver)); destruct (decide (a = b)); subst.
+   - rewrite perm_var,perm_swap_left in H; inversion H; subst; set_solver.
+   - auto.
+Qed.
 
+Lemma app_fresh (a: Name) (m n: Λ): a # App m n → a # m ∧ a # n.
+Proof.
+   intros; apply some_any_iff in H; unfold freshP_a in H.
+   destruct (exist_fresh (support a ∪ support m ∪ support n ∪ support (App m n))) as [w Hw].
+   specialize (H w ltac:(set_solver)); rewrite perm_app in H; inversion H; subst; split;
+   exists w; split; set_solver.
+Qed.
+
+Lemma term_lam_alpha_equiv (a b: Name) (m n: Λ): 
+   Lam a m ≡ Lam b n ↔ ⟦a⟧m ≡ ⟦b⟧n.
+Proof.
+   split; intros.
+   - inversion H; subst; apply alpha_inv_iff; destruct (decide (a = b)); subst.
+      + left; split; auto; destruct (exist_fresh L) as [w Hw]; apply (perm_inj _ _ ⟨b,w⟩).
+        apply H1; assumption.
+      + right.
+        assert (HH: a#n). {
+            destruct (exist_fresh (support a ∪ support b ∪ support m ∪ support n ∪ L)) as [w [[[[]%not_elem_of_union ?]%not_elem_of_union ?]%not_elem_of_union ?]%not_elem_of_union].
+            assert (HH1: ⟨w,b⟩•⟨w,b⟩•n ≡ n). { apply perm_action_duplicate; reflexivity. }
+            assert (HH2: ⟨w,b⟩•⟨w,a⟩•w = a). { rewrite perm_swap_left, perm_swap_neither; auto; apply not_eq_sym,name_neq_fresh_iff,support_fresh; assumption. }
+            rewrite <-HH1; specialize (H1 w ltac:(assumption)). rewrite (swap_perm b w) in H1.
+            rewrite <-HH2,<-H1. rewrite (swap_perm a w). do 2! apply fresh_equivariant; apply support_fresh; assumption.
+         }
+        split; [apply fresh_prod_iff; split |].
+        * apply support_fresh; set_solver.
+        * assumption.
+        * destruct (exist_fresh (support a ∪ support b ∪ support m ∪ support n ∪ L)) as [w [[[[]%not_elem_of_union ?]%not_elem_of_union ?]%not_elem_of_union ?]%not_elem_of_union].
+           specialize (H1 w ltac:(assumption)); apply (perm_inj _ _ ⟨a,w⟩).
+           rewrite perm_swap_distr,perm_swap_left,(perm_swap_neither b a w),(fresh_fixpoint a w n),(swap_perm w b).
+           assumption.
+           assumption.
+           apply support_fresh; assumption.
+           set_solver.
+           set_solver.
+   - apply alpha_inv_iff in H as [[] | []]; subst.
+      + apply AeqAbsC with (L := ∅); intros; apply perm_inj; assumption.
+      + apply AeqAbsC with (L := support a ∪ support b ∪ support m ∪ support n); intros.
+        apply (perm_inj _ _ ⟨a,c⟩).
+        rewrite perm_action_duplicate,perm_swap_distr,perm_swap_neither,perm_swap_right,(fresh_fixpoint a c n),(swap_perm b a).
+        assumption.
+        apply fresh_prod_iff in H as []; assumption.
+        apply support_fresh; set_solver.
+        apply fresh_prod_iff in H as []. apply name_neq_fresh_iff in H. auto.
+        set_solver.
+Qed.
+
+Lemma lam_fresh (a b: Name) (m: Λ): b # Lam a m → a = b ∨ (a ≠ b ∧ b # m).
+Proof.
+   intros; destruct (decide (a = b)); subst.
+   - left; reflexivity.
+   - right; split; auto.
+     destruct (exist_fresh (support a ∪ support b ∪ support m ∪ support (Lam a m))) as [w Hw].
+     exists w; split.
+     + set_solver.
+     + apply some_any_iff in H; unfold freshP_a in H; specialize (H w ltac:(set_solver)).
+       rewrite perm_lam,perm_swap_neither in H.
+       * apply term_lam_alpha_equiv,alpha_inv_name_equiv_iff in H; assumption.
+       * assumption.
+       * set_solver.
+Qed.
+
+Lemma aeq_lam_swap_notin (a b: Name) (t: Λ) : 
+  b ∉ fv (Lam a t) → Lam a t ≡ Lam b (⟨a,b⟩•t).
+Proof.
+  intros; simpl in *; apply not_elem_of_difference in H as []; apply term_lam_alpha_equiv.
+  - apply alpha_rename,support_fresh; assumption.
+  - apply elem_of_singleton in H; subst; rewrite term_action_equal; reflexivity.
+Qed.  
 
 Section InductionAlpha. (* COPELLO's *)
 
-Definition αCompat (P: Term → Prop) : Prop := ∀ m n, aeqCof m n → P m → P n.
+Definition αCompat (P: Λ → Prop): Prop := ∀ m n, m ≡ n → P m → P n.
 
-Lemma perm_ind:
-  ∀ P: Term → Prop, αCompat P →
+Local Lemma perm_ind:
+  ∀ P: Λ → Prop, αCompat P →
     (∀ t, P (Var t)) →
     (∀ m n, P m → P n → P (App m n)) →
     (∀ a m, (∀ p, P (p • m)) → P (Lam a m)) →
     ∀ t, P t.
 Proof.
   intros P Compat Hvar Happ Hlam t.
-  apply (Compat (ɛ • t) _ (gact_id t)). 
-  apply (@Term_ind (fun t => ∀ p, P (p • t))).
+  apply (Compat (ɛ • t) _ (gact_id t)).
+  apply (@Λ_ind (fun t => ∀ p, P (p • t))).
     + intros; rewrite perm_var; apply Hvar.
     + intros; rewrite perm_app; apply Happ; auto.
-    + intros; rewrite perm_lam; apply Hlam; intros.
-      eapply (Compat ((p + p0) • t1)). 
+    + intros a m H p; rewrite perm_lam; apply Hlam; intros.
+      eapply (Compat ((p + p0) • m)). 
       * rewrite gact_compat; reflexivity.
       * apply H.
 Qed.
 
-Lemma aeq_lam_swap_notin (a b: Name) (t: Term) : 
-  b ∉ (fv (Lam a t)) → aeqCof (Lam a t) (Lam b (⟨a,b⟩•t)).
-Proof.
-  intros; simpl in *; apply not_elem_of_difference in H as [].
-  - apply AeqAbsC with (L := fv t ∪ support b ∪ support a); intros; destruct (decide (a = b)); subst.
-    + rewrite perm_swap_distr, perm_swap_left, term_action_equal; reflexivity.
-    + rewrite perm_swap_distr, perm_swap_left, perm_swap_neither; [| set_solver | set_solver].
-      apply term_perm_alpha. rewrite support_spec; set_solver.
-  - apply elem_of_singleton in H; subst; rewrite term_action_equal; reflexivity.
-Qed.
-
-Lemma lam_rename:
-  ∀ P: Term → Prop, αCompat P →
-    ∀ L : NameSet,
+Local Lemma lam_rename (L: NameSet):
+  ∀ P: Λ → Prop, αCompat P →
       (∀ b m, b ∉ L → (∀ p, P (p • m)) → P (Lam b m)) →
       ∀ a m, (∀ p, P (p • m)) → P (Lam a m).
 Proof.
-  intros P Compat L HLam a m Hp. set (c := fresh (support (Lam a m) ∪ L)).
+  intros P Compat HLam a m Hp. set (c := fresh (support (Lam a m) ∪ L)).
   apply (Compat (Lam c (⟨a,c⟩•m))).
   - symmetry. apply aeq_lam_swap_notin. subst c; unfold support, TermSupport; simpl.
     eapply not_elem_of_weaken; [eapply is_fresh | set_solver].
@@ -617,8 +379,8 @@ Proof.
       * apply Hp.
 Qed.
 
-Definition alpha_ind (L : NameSet) :
-  ∀ P: Term → Prop, αCompat P →
+Definition alpha_ind (L: NameSet) :
+  ∀ P: Λ → Prop, αCompat P →
     (∀ a, P (Var a)) →
     (∀ m n, P m → P n → P (App m n)) →
     (∀ a m, a ∉ L → P m → P (Lam a m)) →
@@ -629,7 +391,7 @@ Proof.
   - apply Compat.
   - apply Hvar.
   - apply Happ.
-  - apply lam_rename with L; auto.
+  - apply (lam_rename L); auto.
     intros b m HbL HP; apply HLam.
     + assumption.
     + apply (Compat (ɛ • m)); [apply gact_id | apply HP].
@@ -638,10 +400,150 @@ Qed.
 End InductionAlpha.
 
 Section RecursionAlpha.
-  Context `{Nominal X} (L : NameSet).
-  Context (fvar : Name →ₛ X) (fapp : (X * X) →ₛ X) (flam : [𝔸]X →ₛ X).
-  Context (fvarL : f_supp fvar ⊆ L) (fappL : f_supp fapp ⊆ L) (flamL : f_supp flam ⊆ L).
-  Context (fcb : ∃ a, a ∉ L ∧ ∀ x, a # flam [a]x).
+Context `{Nominal X} (L : NameSet).
+Context (fvar : Name →ₛ X) (fapp : (X * X) →ₛ X) (flam : (Name * X) →ₛ X).
+Context (fvarL : f_supp fvar ⊆ L) (fappL : f_supp fapp ⊆ L) (flamL : f_supp flam ⊆ L).
+Context (fcb: (∃ a, a # flam ∧ ∀ x, a # flam (a,x))).
+
+  Local Lemma fcb_some_any:
+    (∀ a, a # flam → ∀ x, a # (flam (a,x))) ↔ (∃ a, a # flam ∧ ∀ x, a # (flam (a,x))).
+  Proof.
+    clear fcb; split; intros.
+    - destruct (exist_fresh (support flam)) as [w Hw]; exists w; split.
+      + apply support_fresh; assumption.
+      + apply H1, support_fresh; auto.
+    - destruct H1 as [w [H1w H2w]]; destruct (decide (a = w)).
+      + subst; auto.
+      + specialize (H2w (⟨a,w⟩•x)). apply (fresh_equivariant ⟨a,w⟩) in H2w.
+        rewrite perm_swap_right,fun_equivar,prod_act,perm_swap_right,
+                fresh_fixpoint,perm_action_duplicate in H2w; assumption.
+  Qed.
+
+  Local Lemma alpha_flam_equiv (a b: Name) (x y: X): 
+    a # flam → b # flam → ⟦a⟧x ≈α ⟦b⟧y → flam (a,x) ≡ flam (b,y).
+  Proof.
+    intros. 
+    destruct (exist_fresh (support a ∪ support b ∪ support x ∪ support y ∪ support flam ∪ support (flam (a,x)) ∪ support (flam (b,y)))) as [c ?].
+    apply not_elem_of_union in H4 as [[[[[[]%not_elem_of_union ?]%not_elem_of_union ?]%not_elem_of_union ?]%not_elem_of_union ?]%not_elem_of_union ?].
+    rewrite <-(fresh_fixpoint c a (flam (a,x))), <-(fresh_fixpoint c b (flam (b,y))); auto.
+    rewrite !fun_equivar, !(fresh_fixpoint _ _ flam), !prod_act, !perm_swap_right; try (apply fsupp_equiv); try auto.
+    unfold equiv,prod_equiv,prod_relation; simpl; split.
+      + reflexivity.
+      + apply alpha_some_any in H3; apply H3; repeat split; apply support_fresh; auto.
+      + apply support_fresh; assumption.
+      + apply support_fresh; assumption.
+      + apply support_fresh; assumption.
+      + eapply fcb_some_any in fcb; eauto.
+      + apply support_fresh; assumption.
+      + eapply fcb_some_any in fcb; eauto.
+  Qed.
+
+  Lemma perm_swap_equal (a b: Name) (x: X): ⟨a,b⟩ • x ≡ ⟨b,a⟩ • x.
+  Proof. rewrite swap_perm; reflexivity. Qed.
+
+  Definition _flam : [𝔸]X →ₛ X.
+    refine (
+      λₛ⟦support flam⟧ (ax: [𝔸]X), 
+        let h: Name →ₛ X := λₛ⟦support (ax.(name)) ∪ support (ax.(term)) ∪ support flam⟧ c, 
+        (flam (c, ⟨ax.(name),c⟩ • ax.(term))) in freshF h
+    ).
+  Proof.
+    all: swap 1 2.
+    - intros w z Hw Hz [a x]; unfold freshF.
+      set (g := (λₛ⟦_⟧ c : Name, flam (c, ⟨name (⟨w,z⟩ • ⟦a⟧x),c⟩ • term (⟨w,z⟩ • ⟦a⟧x)))).
+      set (h := (λₛ⟦_⟧ c : Name, flam (c, ⟨name ⟦a⟧x,c⟩ • term ⟦a⟧x))).
+      destruct (exist_fresh (L ∪ support flam ∪ support w ∪ support z ∪ support x ∪ support h ∪ support g)) as [c Hc].
+      erewrite (freshness_theorem_inj g _ (fresh (support g)) c), (freshness_theorem_inj h _ (fresh (support h)) c);
+      try (apply fresh_support_fresh); try (apply support_fresh; set_solver).
+      subst g h; simpl.
+      rewrite fun_equivar, support_spec, !prod_act; auto.
+      assert (HH: ∀ (a b c : Name), perm_swap ⟨a,b⟩ c = ⟨a,b⟩ • c). { intros; unfold action, name_action; reflexivity. }
+      rewrite perm_swap_distr. rewrite (HH w z c), (HH w z (⟨w,z⟩ • a)).
+      rewrite !perm_action_duplicate, !(name_action_neither w z c). reflexivity. 
+      apply not_elem_of_union in Hc as [[[[[? ?]%not_elem_of_union ?]%not_elem_of_union ?]%not_elem_of_union ?]%not_elem_of_union ?].
+      apply name_neq_fresh_iff, support_fresh; assumption.
+      apply not_elem_of_union in Hc as [[[[[? ?]%not_elem_of_union ?]%not_elem_of_union ?]%not_elem_of_union ?]%not_elem_of_union ?].
+      apply name_neq_fresh_iff, support_fresh; assumption.
+    - intros x y Hxy; unfold freshF; cbn zeta; set (w := fresh _); set (z := fresh _).
+      set (g := (λₛ⟦ _ ⟧ c : Name, flam (c, ⟨name x,c⟩ • term x))).
+      set (h := (λₛ⟦ _ ⟧ c : Name, flam (c, ⟨name y,c⟩ • term y))).
+      destruct x as [a x]; destruct y as [b y].
+      destruct (exist_fresh (L ∪ support flam ∪ support w ∪ support z ∪ support h ∪ support g ∪ support x ∪ support y)) as [c Hc].
+      erewrite (freshness_theorem_inj g _ w c), (freshness_theorem_inj h _ z c);
+      try (apply fresh_support_fresh); try (apply support_fresh; set_solver).
+      simpl. apply not_elem_of_union in Hc as [[[[[[[]%not_elem_of_union ?]%not_elem_of_union ?]%not_elem_of_union ?]%not_elem_of_union ?]%not_elem_of_union ?]%not_elem_of_union ?].
+      apply alpha_flam_equiv; try (apply support_fresh; assumption).
+      pose proof (@Equivalence_Transitive _ _ alpha_equivalence_e) as T; pose proof (@Equivalence_Symmetric _ _ alpha_equivalence_e) as S.
+      transitivity (⟦a⟧x). symmetry. apply alpha_rename, support_fresh; assumption.
+      transitivity (⟦b⟧y). apply Hxy. apply alpha_rename, support_fresh; assumption.
+    Unshelve.
+      + simpl; destruct (exist_fresh (support g ∪ support flam)) as [k Hk]; exists k; split.
+        * apply support_fresh; set_solver.
+        * eapply fcb_some_any in fcb; eauto; apply support_fresh; set_solver. 
+      + simpl; destruct (exist_fresh (support h ∪ support flam)) as [k Hk]; exists k; split.
+        * apply support_fresh; set_solver.
+        * eapply fcb_some_any in fcb; eauto; apply support_fresh; set_solver.
+      + typeclasses eauto.
+      + typeclasses eauto.
+      + typeclasses eauto.
+      + assumption.
+      + typeclasses eauto.
+      + intros w z Hw Hz c.
+        rewrite <-(fresh_fixpoint w z flam) at 2;  try (apply support_fresh; set_solver).
+        rewrite fsupp_action, <-perm_inv, prod_act. apply gact_proper. reflexivity.
+        apply fsupp_equiv. unfold equiv,prod_equiv,prod_relation; simpl; split.
+        * reflexivity.
+        * assert (HH: ∀ (a b c : Name), perm_swap ⟨a,b⟩ c = ⟨a,b⟩ • c). { intros; unfold action, name_action; reflexivity. }
+          rewrite perm_swap_distr, (HH w z (name ax)), (HH w z c).
+          rewrite (name_action_neither w z (name ax)), (support_spec (term ax) w z).
+          reflexivity. set_solver. set_solver. 
+          symmetry. apply name_neq_fresh_iff, support_fresh. set_solver. 
+          symmetry. apply name_neq_fresh_iff, support_fresh. set_solver.
+      + simpl; destruct (exist_fresh (support g ∪ support flam)) as [k Hk]; exists k; split.
+        * apply support_fresh; set_solver.
+        * eapply fcb_some_any in fcb; eauto; apply support_fresh; set_solver.
+      + simpl; destruct (exist_fresh (support h ∪ support flam)) as [k Hk]; exists k; split.
+        * apply support_fresh; set_solver.
+        * eapply fcb_some_any in fcb; eauto; apply support_fresh; set_solver.
+  Defined.
+
+  Section _flamProperties.
+
+  Local Lemma flam_abs_eq_flam_support: support flam = support _flam.
+  Proof. reflexivity. Qed.
+
+  (* TODO: Better name *)
+  Local Lemma efs (a: Name): a ∉ support flam → ∀ x: X, flam (a,x) ≡ _flam ⟦a⟧x.
+  Proof. 
+    intros. simpl. set (w := fresh _). apply alpha_flam_equiv.
+    - apply support_fresh; assumption.
+    - subst w; unfold support; simpl; apply support_fresh; apply not_elem_of_weaken with (Y := name_support a ∪ Spt x ∪ fun_supp_support flam).
+      apply is_fresh. set_solver.
+    - apply alpha_rename, support_fresh; subst w; unfold support; simpl.
+      apply not_elem_of_weaken with (Y := name_support a ∪ Spt x ∪ fun_supp_support flam).
+      apply is_fresh. set_solver.
+  Qed.
+
+  Local Lemma ft_flam (Fm: Perm →ₛ X) (a: Name) (p: Perm) (Sp: NameSet): 
+    ∃ c: Name, (c ∉ Sp) ∧ c # _flam ⟦c⟧(Fm (⟨a,c⟩ + p)).
+  Proof.
+    destruct (exist_fresh (Sp ∪ support _flam)) as [w Hw]; exists w; split.
+    - apply not_elem_of_union in Hw as []; assumption.
+    - rewrite <-efs; rewrite <-flam_abs_eq_flam_support in *.
+      + destruct (exist_fresh (support flam)) as [d Hd].
+        rewrite <-(fresh_fixpoint d w flam),fsupp_action,<-perm_inv,prod_act,name_action_right.
+        pose proof fcb_some_any as []. specialize (H2 fcb). apply support_fresh in Hd.
+        specialize (H2 d Hd (⟨d,w⟩•(Fm (⟨a,w⟩ + p)))).
+        apply (fresh_equivariant ⟨d,w⟩) in H2; rewrite perm_swap_left in H2.
+        apply H2.
+        apply support_fresh; auto.
+        apply support_fresh; apply not_elem_of_union in Hw as []; assumption.
+      + apply not_elem_of_union in Hw as []; assumption.
+  Qed.
+
+  End _flamProperties.
+
+  Opaque _flam. (* Don't look inside _flam *)
 
   Definition g_var (a: Name): Perm →ₛ X.
     refine (λₛ⟦L ∪ support a⟧ p : Perm, fvar (p • a)).
@@ -655,15 +557,8 @@ Section RecursionAlpha.
           try (apply support_fresh; set_solver); reflexivity.
   Defined.
 
-  Definition g_var_term: Name →ₛ X.
-    refine (λₛ⟦L⟧ a : Name, fvar a).
-  Proof.
-    intros ? ? Ha Hb ?; rewrite <-(support_spec fvar a b),<-fun_equivar,perm_action_duplicate,
-    support_spec; auto.
-  Defined.
-
   Definition g_app (Fm Fn: Perm →ₛ X): Perm →ₛ X.
-    refine (λₛ⟦ L ∪ support Fm ∪ support Fn⟧ p, fapp (Fm p, Fn p)).
+    refine (λₛ⟦L ∪ support Fm ∪ support Fn⟧ p, fapp (Fm p, Fn p)).
   Proof.
     - intros ? ? HH; rewrite HH; reflexivity.
     - intros w z [[]%not_elem_of_union]%not_elem_of_union [[]%not_elem_of_union]%not_elem_of_union p.
@@ -673,134 +568,161 @@ Section RecursionAlpha.
       rewrite fresh_fixpoint; try (apply support_fresh; set_solver); reflexivity.
   Defined.
 
-  Definition g_app_term (Fm Fn: Term →ₛ X): (Term * Term) →ₛ X.
-    refine (λₛ⟦ L ∪ support Fm ∪ support Fn⟧ mn, fapp (Fm mn.1, Fn mn.2)).
-  Proof.
-    - intros [x y] [x' y'] [H1 H2]; simpl in *; rewrite H1,H2; reflexivity.
-    - intros a b [[]%not_elem_of_union]%not_elem_of_union [[]%not_elem_of_union]%not_elem_of_union [m n]; simpl.
-      rewrite <-(fresh_fixpoint a b Fm) at 1; try (apply support_fresh; set_solver); rewrite <-(fresh_fixpoint a b Fn) at 1; try (apply support_fresh; set_solver).
-      rewrite <-!(fun_equivar),<-prod_act; rewrite <-(support_spec fapp a b),<-fun_equivar,perm_action_duplicate at 1; auto.
-  Defined.
-
-  Local Lemma ft_flam (Fm: Perm →ₛ X) a p (Sp: NameSet): 
-    ∃ c : Name, (c ∉ Sp) ∧ c # flam [c](Fm (⟨a,c⟩ + p)).
-  Proof.
-    destruct (exist_fresh (Sp ∪ support flam)) as [w Hw]; exists w; split.
-    - set_solver.
-    - destruct fcb as [d [? Hd]].
-      specialize (Hd (⟨d,w⟩•(Fm (⟨a,w⟩ + p)))).
-      apply ((fresh_equivariant ⟨d,w⟩ _ _)) in Hd; rewrite perm_swap_left in Hd.
-      rewrite <-(fresh_fixpoint d w flam), fsupp_action, <-perm_inv, nabs_action, name_action_right;
-      [apply Hd | |]; apply support_fresh; set_solver.
-  Qed.
-
-  Definition g_lam (a: Name) (m: Term) (Fm: Perm →ₛ X): Perm →ₛ X.
+  Definition g_lam (a: Name) (m: Λ) (Fm: Perm →ₛ X): Perm →ₛ X.
     refine (
       λₛ⟦ L ∪ support a ∪ support (Fm) ⟧ p,
-        let h: Name →ₛ X := λₛ⟦L ∪ support flam ∪ support a ∪ support m ∪ support (Fm) ∪ support p⟧ a', 
-          (flam [a'](Fm (⟨a,a'⟩ + p))) in freshF h
+        let h: Name →ₛ X := λₛ⟦L ∪ support _flam ∪ support a ∪ support m ∪ support (Fm) ∪ support p⟧ a', 
+          (_flam ⟦a'⟧(Fm (⟨a,a'⟩ + p))) in freshF h
     ).
     all: swap 1 2.
     - intros w z Hw Hz p; unfold freshF; cbn zeta.
-      set (g := (λₛ⟦ _ ⟧ a' : Name, flam [a'](Fm (⟨ a, a' ⟩ + (⟨ w, z ⟩ • p))))).
-      set (h := (λₛ⟦ _ ⟧ a' : Name, flam [a'](Fm (⟨ a, a' ⟩ + p)))).
-      destruct (exist_fresh (L ∪ support flam ∪ support a ∪ support m ∪ support (Fm) ∪ support w ∪ support z ∪ support (⟨ w, z ⟩ • p) ∪ support p)) as [b Hb].
-      rewrite (freshness_theorem2 g (fresh (support g)) b), (freshness_theorem2 h (fresh (support h)) b);
+      set (g := (λₛ⟦ _ ⟧ a' : Name, _flam ⟦a'⟧(Fm (⟨ a, a' ⟩ + (⟨ w, z ⟩ • p))))).
+      set (h := (λₛ⟦ _ ⟧ a' : Name, _flam ⟦a'⟧(Fm (⟨ a, a' ⟩ + p)))).
+      destruct (exist_fresh (L ∪ support _flam ∪ support a ∪ support m ∪ support (Fm) ∪ support w ∪ support z ∪ support (⟨ w, z ⟩ • p) ∪ support p)) as [b Hb].
+      erewrite (freshness_theorem_inj g _ (fresh (support g)) b), (freshness_theorem_inj h _ (fresh (support h)) b);
       try (apply fresh_support_fresh); try (apply support_fresh; subst h g; unfold support at 1; simpl; split_union; repeat (apply not_elem_of_union; split; try eauto)).
-      all: swap 1 2. all: swap 2 3; try (subst; simpl; apply ft_flam).
-      + subst g h; simpl.
-        assert (HH: flam [b](Fm (⟨a,b⟩+(⟨w,z⟩•p))) ≡ flam [b]((⟨w,z⟩•(Fm)) (⟨w,z⟩•⟨a,b⟩+p))). {
-        apply fsupp_equiv, nabs_inv;
-        rewrite perm_distr_1, perm_distr,<-(fresh_fixpoint w z (Fm)) at 1;
-        try reflexivity; try (apply support_fresh); set_solver.
-        } rewrite HH; clear HH.
-        rewrite <-(fresh_fixpoint w z b) at 1; try (apply support_fresh; set_solver).
-        assert (HH: flam [⟨w,z⟩•b]((⟨w,z⟩•(Fm)) (⟨w,z⟩•⟨a,b⟩+p)) ≡ flam ([⟨w,z⟩•b](⟨w,z⟩•(Fm (⟨a,b⟩+p))))). {
-        apply fsupp_equiv, nabs_inv; rewrite fun_equivar; reflexivity.
-        } rewrite HH; clear HH.
-        rewrite <-nabs_action,<-fsupp_action, fresh_fixpoint; try (apply support_fresh; set_solver);
-        reflexivity.
-      - intros x y Hxy; unfold freshF; cbn zeta; set (a' := fresh _); set (b' := fresh _);
-        set (g := (λₛ⟦ _ ⟧ _ : Name, flam [_](Fm (⟨ a, _ ⟩ + x))));
-        set (h := (λₛ⟦ _ ⟧ _' : Name, flam [_](Fm (⟨ a, _ ⟩ + y))));
-        destruct (exist_fresh (L ∪ support flam ∪ support a ∪ support m ∪ support (Fm) ∪ support x ∪ support y ∪ support a' ∪ support b')) as [c Hc];
-        rewrite (freshness_theorem2 g a' c), (freshness_theorem2 h b' c);
-        try (apply fresh_support_fresh); try (apply support_fresh; subst h g; unfold support at 1; simpl; split_union; repeat (apply not_elem_of_union; split; try eauto));
-        try (subst; simpl; apply ft_flam);
-        simpl; apply fsupp_equiv, nabs_inv, fsupp_equiv, grp_op_proper; auto.
+      (* all: swap 1 2. all: swap 2 3; try (subst; simpl; apply ft_flam). *)
+      subst g h; simpl.
+      assert (HH: _flam ⟦b⟧(Fm (⟨a,b⟩+(⟨w,z⟩•p))) ≡ _flam ⟦b⟧((⟨w,z⟩•(Fm)) (⟨w,z⟩•⟨a,b⟩+p))). {
+      apply fsupp_equiv, nabs_inv;
+      rewrite perm_distr_1, perm_distr,<-(fresh_fixpoint w z (Fm)) at 1;
+      try reflexivity; try (apply support_fresh).
+      apply not_elem_of_union in Hw as [[]%not_elem_of_union ?]; assumption.
+      apply not_elem_of_union in Hz as [[]%not_elem_of_union ?]; assumption.
+      apply not_elem_of_union in Hw as [[]%not_elem_of_union ?]; apply name_neq_fresh_iff, support_fresh; assumption.
+      apply not_elem_of_union in Hb as [[[[]%not_elem_of_union ?]%not_elem_of_union ?]%not_elem_of_union ?]; symmetry; apply name_neq_fresh_iff, support_fresh; assumption.
+      apply not_elem_of_union in Hz as [[]%not_elem_of_union ?]; apply name_neq_fresh_iff, support_fresh; assumption.
+      apply not_elem_of_union in Hb as [[[]%not_elem_of_union ?]%not_elem_of_union ?]; symmetry; apply name_neq_fresh_iff, support_fresh; assumption.
+      } rewrite HH; clear HH.
+      rewrite <-(fresh_fixpoint w z b) at 1.
+      all: swap 1 2.
+      apply not_elem_of_union in Hb as [[[[]%not_elem_of_union ?]%not_elem_of_union ?]%not_elem_of_union ?]; apply name_fresh_iff, support_fresh; assumption.
+      all: swap 1 2.
+      apply not_elem_of_union in Hb as [[[]%not_elem_of_union ?]%not_elem_of_union ?]; apply name_fresh_iff, support_fresh; assumption.
+      assert (HH: _flam ⟦⟨w,z⟩•b⟧((⟨w,z⟩•(Fm)) (⟨w,z⟩•⟨a,b⟩+p)) ≡ _flam (⟦⟨w,z⟩•b⟧(⟨w,z⟩•(Fm (⟨a,b⟩+p))))). {
+      apply fsupp_equiv, nabs_inv; rewrite fun_equivar; reflexivity.
+      } rewrite HH; clear HH.
+      rewrite <-nabs_action,<-fsupp_action, fresh_fixpoint. reflexivity.
+      apply not_elem_of_union in Hw as [[]%not_elem_of_union ?]; apply support_fresh; rewrite <-flam_abs_eq_flam_support.
+      apply not_elem_of_weaken with L; assumption.
+      apply not_elem_of_union in Hz as [[]%not_elem_of_union ?]; apply support_fresh; rewrite <-flam_abs_eq_flam_support.
+      apply not_elem_of_weaken with L; assumption.
+    - intros x y Hxy; unfold freshF; cbn zeta; set (a' := fresh _); set (b' := fresh _);
+      set (g := (λₛ⟦ _ ⟧ _ : Name, _flam ⟦_⟧(Fm (⟨ a, _ ⟩ + x))));
+      set (h := (λₛ⟦ _ ⟧ _' : Name, _flam ⟦_⟧(Fm (⟨ a, _ ⟩ + y))));
+      destruct (exist_fresh (L ∪ support _flam ∪ support a ∪ support m ∪ support (Fm) ∪ support x ∪ support y ∪ support a' ∪ support b')) as [c Hc];
+      erewrite (freshness_theorem_inj g _ a' c), (freshness_theorem_inj h _ b' c);
+      try (apply fresh_support_fresh); try (apply support_fresh; subst h g; unfold support at 1; simpl; split_union; repeat (apply not_elem_of_union; split; try eauto)).
+      simpl; apply fsupp_equiv, nabs_inv, fsupp_equiv, grp_op_proper; auto.
   Unshelve.
-    eabstract(
-      intros w z Hw Hz b;
-      rewrite <-(fresh_fixpoint w z flam) at 2; try (apply support_fresh; set_solver);
-      rewrite fsupp_action, <-perm_inv, nabs_action; apply gact_proper, fsupp_equiv; auto;
-      rewrite (fun_equivar (⟨w,z⟩) (Fm)), (fresh_fixpoint w z (Fm)); try (apply support_fresh; set_solver);
-      rewrite perm_distr_3; set_solver
-    ).
+      (* Make these proof terms opaque to reduce term size. *)
+      eabstract(
+        intros w z Hw Hz b;
+        apply not_elem_of_union in Hw as [[[[[]%not_elem_of_union ?]%not_elem_of_union ?]%not_elem_of_union ?]%not_elem_of_union ?];
+        apply not_elem_of_union in Hz as [[[[[]%not_elem_of_union ?]%not_elem_of_union ?]%not_elem_of_union ?]%not_elem_of_union ?];
+        rewrite <-(fresh_fixpoint w z _flam) at 2; try (apply support_fresh; assumption);
+        rewrite fsupp_action, <-perm_inv, nabs_action; apply gact_proper, fsupp_equiv; auto;
+        rewrite (fun_equivar (⟨w,z⟩) (Fm)), (fresh_fixpoint w z (Fm)); try (apply support_fresh; assumption);
+        rewrite perm_distr_3; try (apply name_neq_fresh_iff, support_fresh); try assumption; reflexivity).
+      eabstract(
+        simpl; destruct (exist_fresh (support g ∪ support flam)) as [k []%not_elem_of_union]; exists k; split;
+        [apply support_fresh; assumption | pose proof fcb_some_any as [? hh]; specialize (hh fcb); rewrite <-efs; [eapply hh; apply support_fresh; assumption | assumption]]
+      ).
+      eabstract(
+        simpl; destruct (exist_fresh (support h ∪ support flam)) as [k []%not_elem_of_union]; exists k; split;
+        [apply support_fresh; assumption | pose proof fcb_some_any as [? hh]; specialize (hh fcb); rewrite <-efs; [eapply hh; apply support_fresh; assumption | assumption]]
+      ).
+      eabstract(
+        simpl; destruct (exist_fresh (support g ∪ support flam)) as [k []%not_elem_of_union]; exists k; split;
+        [apply support_fresh; assumption | pose proof fcb_some_any as [? hh]; specialize (hh fcb); rewrite <-efs; [eapply hh; apply support_fresh; assumption | assumption]]
+      ).
+      eabstract(
+        simpl; destruct (exist_fresh (support h ∪ support flam)) as [k []%not_elem_of_union]; exists k; split;
+        [apply support_fresh; assumption | pose proof fcb_some_any as [? hh]; specialize (hh fcb); rewrite <-efs; [eapply hh; apply support_fresh; assumption | assumption]]
+      ).
   Defined.
 
-  Fixpoint perm_alpha_rec (t : Term) : Perm →ₛ X :=
+  Fixpoint perm_alpha_rec (t: Λ): Perm →ₛ X :=
   match t with
     | Var a => g_var a
     | App m n => g_app (perm_alpha_rec m) (perm_alpha_rec n)
     | Lam a m => g_lam a m (perm_alpha_rec m)
   end.
 
-  Lemma perm_alpha_rec_var a:
+  Lemma perm_alpha_rec_var (a: Name):
     perm_alpha_rec (Var a) = g_var a.
   Proof. simpl; reflexivity. Qed.
 
-  Lemma perm_alpha_rec_app (m n: Term):
+  Lemma perm_alpha_rec_app (m n: Λ):
     perm_alpha_rec (App m n) = g_app (perm_alpha_rec m) (perm_alpha_rec n).
   Proof. simpl; reflexivity. Qed.
 
-  Lemma perm_alpha_rec_lam a (m: Term):
+  Lemma perm_alpha_rec_lam (a: Name) (m: Λ):
     perm_alpha_rec (Lam a m) = g_lam a m (perm_alpha_rec m).
   Proof. simpl; reflexivity. Qed.
 
-  Lemma alpha_rec_perm (t: Term):
+  Lemma alpha_rec_perm (t: Λ):
     ∀ (p q: Perm), perm_alpha_rec t (q + p) ≡ perm_alpha_rec (q • t) p.
   Proof. 
     induction t; intros.
     - simpl; rewrite gact_compat; reflexivity.
-  Admitted.
-
+    - simpl; rewrite IHt1,IHt2; reflexivity.
+    - Opaque freshF. rewrite perm_lam; simpl.
+      set (f := λₛ⟦ _ ⟧ a' : Name, _flam ⟦_⟧(_)); set (g := λₛ⟦ _ ⟧ a' : Name, _flam ⟦_⟧(_)).
+      destruct (exist_fresh (support f ∪ support g ∪ support q)) as [w [[]%not_elem_of_union]%not_elem_of_union].
+      erewrite <-!(freshness_theorem _ _ w); try (apply support_fresh; auto).
+      simpl; apply fsupp_equiv,nabs_inv.
+      rewrite grp_assoc,perm_comm_distr,(perm_notin_domain_id _ w),<-grp_assoc,IHt; try reflexivity.
+      auto. Unshelve.
+      + subst f; simpl. pose proof (ft_flam (perm_alpha_rec t0) t (q + p) (L ∪ support _flam ∪ support t ∪ support t0 ∪ support (perm_alpha_rec t0) ∪ support (q + p))) as [w' []]. 
+        exists w'. split.
+        * apply support_fresh; unfold support. simpl. auto.
+        * auto.
+      + subst g; simpl. pose proof (ft_flam (perm_alpha_rec (q • t0)) (q•t) p (L ∪ support _flam ∪ support (q • t) ∪ support (q • t0) ∪ support (perm_alpha_rec (q • t0)) ∪ support p)) as [w' []].
+        exists w'. split.
+        * apply support_fresh; unfold support; simpl; auto.
+        * auto.
+      Transparent freshF.
+  Qed.
+  
 (* perhaps can be made simpler *)
-  Theorem perm_alpha_rec_respectfull (m n : Term) :
-    aeqCof m n → perm_alpha_rec m ≡ perm_alpha_rec n.
+  Theorem perm_alpha_rec_respectfull (m n: Λ):
+    m ≡α n → perm_alpha_rec m ≡ perm_alpha_rec n.
   Proof.
     induction 1.
     - simpl; unfold g_var; reflexivity.
-    - simpl; unfold g_app; unfold equiv, fun_supp_equiv; intro p; simpl.
-      rewrite IHaeqCof1, IHaeqCof2; reflexivity.
+    - simpl; unfold g_app; unfold equiv, fun_supp_equiv; intro p; simpl. rewrite IHaeqCof1, IHaeqCof2; reflexivity.
     - simpl; unfold g_lam, equiv, fun_supp_equiv; intros p; simpl.
-      set (s1 := L ∪ support flam ∪ support a ∪ support m ∪ support (perm_alpha_rec m) ∪ support p);
-      set (s2 := L ∪ support flam ∪ support b ∪ support n ∪ support (perm_alpha_rec n) ∪ support p).
-      set (h1 := (λₛ⟦ s1 ⟧ a' : Name, flam [a'](perm_alpha_rec m (⟨ a, a' ⟩ + p))));
-      set (h2 := (λₛ⟦ s2 ⟧ a' : Name, flam [a'](perm_alpha_rec n (⟨ b, a' ⟩ + p)))).
-      assert (HH1: flam [fresh (support h1)](perm_alpha_rec m (⟨ a, fresh (support h1) ⟩ + p)) = h1 (fresh (support h1))).
+      set (s1 := L ∪ support _flam ∪ support a ∪ support m ∪ support (perm_alpha_rec m) ∪ support p);
+      set (s2 := L ∪ support _flam ∪ support b ∪ support n ∪ support (perm_alpha_rec n) ∪ support p).
+      set (h1 := (λₛ⟦ s1 ⟧ a' : Name, _flam ⟦a'⟧(perm_alpha_rec m (⟨ a, a' ⟩ + p))));
+      set (h2 := (λₛ⟦ s2 ⟧ a' : Name, _flam ⟦a'⟧(perm_alpha_rec n (⟨ b, a' ⟩ + p)))).
+      assert (HH1: _flam ⟦fresh (support h1)⟧(perm_alpha_rec m (⟨ a, fresh (support h1) ⟩ + p)) = h1 (fresh (support h1))).
       { subst h1 s1; reflexivity. }
-      assert (HH2: flam [fresh (support h2)](perm_alpha_rec n (⟨ b, fresh (support h2) ⟩ + p)) = h2 (fresh (support h2))).
+      assert (HH2: _flam ⟦fresh (support h2)⟧(perm_alpha_rec n (⟨ b, fresh (support h2) ⟩ + p)) = h2 (fresh (support h2))).
       { subst h2 s2; reflexivity. }
       rewrite HH1, HH2; clear HH1 HH2.
       destruct (exist_fresh (L0 ∪ support h2 ∪ support h1)) as [w Hw].
-      (* destruct (exist_fresh (support a ∪ support b ∪ atms m ∪ atms n ∪ support h2 ∪ support h1 ∪ support flam ∪ L ∪ L0)) as [w Hw]. *)
-      rewrite (freshness_theorem2 h1 (fresh (support h1)) w), (freshness_theorem2 h2 (fresh (support h2)) w).
+      erewrite (freshness_theorem_inj h1 _ (fresh (support h1)) w), (freshness_theorem_inj h2 _ (fresh (support h2)) w).
       + subst h1 h2; simpl; apply fsupp_equiv; rewrite !alpha_rec_perm.
         apply name_abstraction_inv; left; split; auto.
         rewrite H2. reflexivity. apply not_elem_of_union in Hw as [[]%not_elem_of_union]. assumption.
-      + apply ft_flam.
-      + apply fresh_support_fresh.
+      + apply fresh_support_fresh. 
       + apply support_fresh. apply not_elem_of_union in Hw as [[]%not_elem_of_union]. assumption.
-      + apply ft_flam.
-      + apply fresh_support_fresh.
+      + apply fresh_support_fresh. 
       + apply support_fresh. apply not_elem_of_union in Hw as [[]%not_elem_of_union]. assumption.
+  Unshelve.
+      simpl; destruct (exist_fresh (support h1 ∪ support flam)) as [k []%not_elem_of_union]; exists k; split;
+        [apply support_fresh; assumption | pose proof fcb_some_any as [? hh]; specialize (hh fcb); rewrite <-efs; [eapply hh; apply support_fresh; assumption | assumption]].
+      simpl; destruct (exist_fresh (support h2 ∪ support flam)) as [k []%not_elem_of_union]; exists k; split;
+        [apply support_fresh; assumption | pose proof fcb_some_any as [? hh]; specialize (hh fcb); rewrite <-efs; [eapply hh; apply support_fresh; assumption | assumption]].
   Qed.
 
   Instance: Proper (aeqCof ==> equiv) (perm_alpha_rec).
   Proof. repeat intro; apply perm_alpha_rec_respectfull; assumption. Qed.
 
-  Lemma perm_alpha_rec_supported a b t :
-  ∀ p, a ∉ (L ∪ support p) → b ∉ (L ∪ support p) → ⟨a,b⟩•(perm_alpha_rec (⟨a,b⟩•t)) p ≡ perm_alpha_rec t p.
+  Lemma perm_alpha_rec_supported (a b: Name) (t: Λ):
+    ∀ p: Perm, a ∉ (L ∪ support p) → b ∉ (L ∪ support p) → ⟨a,b⟩•(perm_alpha_rec (⟨a,b⟩•t)) p ≡ perm_alpha_rec t p.
   Proof.
     set (P := fun t => ∀ p : Perm, a ∉ (L ∪ support p) → b ∉ (L ∪ support p) → ⟨ a, b ⟩ • perm_alpha_rec (⟨ a, b ⟩ • t) p ≡ perm_alpha_rec t p).
     apply (alpha_ind (L ∪ support a ∪ support b) P); subst P.
@@ -808,11 +730,11 @@ Section RecursionAlpha.
       transitivity (⟨ a, b ⟩ • perm_alpha_rec (⟨ a, b ⟩ • m) p).
       + apply perm_inj; apply H5,term_perm_alpha; symmetry; assumption.
       + transitivity (perm_alpha_rec m p). apply H2; assumption. apply H5. assumption. 
-    - simpl; intros x p ? ?. rewrite fun_equivar, support_spec. rewrite perm_comm,perm_action_duplicate. reflexivity.
-      + set_solver.
-      + set_solver.
-      + set_solver.
-      + set_solver.
+    - simpl; intros x p ? ?. rewrite not_elem_of_union in H1,H2. destruct H1,H2. rewrite fun_equivar, support_spec. rewrite perm_comm,perm_action_duplicate. reflexivity.
+      + assumption.
+      + assumption.
+      + eapply not_elem_of_weaken. eapply H1. assumption.
+      + eapply not_elem_of_weaken. eapply H2. assumption.
     - intros m n IHt1 IHt2. Opaque perm_alpha_rec. simpl in *. Transparent perm_alpha_rec.
       intros p ? ?. rewrite action_app,perm_alpha_rec_app. simpl.
       rewrite fun_equivar, support_spec, prod_act. apply fsupp_equiv. split; simpl; auto.
@@ -822,11 +744,11 @@ Section RecursionAlpha.
       intros IHt p aL bL.
       rewrite perm_lam,!perm_alpha_rec_lam; unfold g_lam.
       Opaque freshF. simpl. Transparent freshF.
-      set (h := λₛ⟦ _ ⟧ a' : Name, flam [a'](perm_alpha_rec (⟨ a, b ⟩ • m) (⟨ ⟨ a, b ⟩ • c, a' ⟩ + p))).
-      set (g := λₛ⟦ _ ⟧ a' : Name, flam [a'](perm_alpha_rec m (⟨ c, a' ⟩ + p))).
+      set (h := λₛ⟦ _ ⟧ a' : Name, _flam ⟦a'⟧(perm_alpha_rec (⟨ a, b ⟩ • m) (⟨ ⟨ a, b ⟩ • c, a' ⟩ + p))).
+      set (g := λₛ⟦ _ ⟧ a' : Name, _flam ⟦a'⟧(perm_alpha_rec m (⟨ c, a' ⟩ + p))).
       unfold freshF.
       destruct (exist_fresh (support g ∪ support h ∪ support a ∪ support b)) as [w Hw].
-      rewrite (freshness_theorem2 h (fresh (support h)) w), (freshness_theorem2 g (fresh (support g)) w).
+      erewrite (freshness_theorem_inj h _ (fresh (support h)) w), (freshness_theorem_inj g _ (fresh (support g)) w).
       + simpl; rewrite fun_equivar, support_spec, nabs_action, support_spec.
         apply fsupp_equiv,nabs_inv. rewrite name_action_neither. apply IHt.
         * apply not_elem_of_union in aL as []; apply not_elem_of_union; split. assumption. apply notin_support_comp_perm. split.
@@ -845,42 +767,42 @@ Section RecursionAlpha.
         * apply not_elem_of_union in Hw as [[[]%not_elem_of_union ?]%not_elem_of_union ?]. set_solver.
         * apply not_elem_of_union in aL as []; apply not_elem_of_weaken with (Y := L). auto. assumption.
         * apply not_elem_of_union in bL as []; apply not_elem_of_weaken with (Y := L). auto. assumption.
-      + apply ft_flam.
       + apply fresh_support_fresh.
       + apply not_elem_of_union in Hw as [[[]%not_elem_of_union ?]%not_elem_of_union ?]. apply support_fresh. set_solver.
-      + apply ft_flam.
       + apply fresh_support_fresh.
       + apply not_elem_of_union in Hw as [[[]%not_elem_of_union ?]%not_elem_of_union ?]. apply support_fresh. set_solver.
+  Unshelve.
+    simpl; destruct (exist_fresh (support h ∪ support flam)) as [k []%not_elem_of_union]; exists k; split;
+        [apply support_fresh; assumption | pose proof fcb_some_any as [? hh]; specialize (hh fcb); rewrite <-efs; [eapply hh; apply support_fresh; assumption | assumption]].
+    simpl; destruct (exist_fresh (support g ∪ support flam)) as [k []%not_elem_of_union]; exists k; split;
+        [apply support_fresh; assumption | pose proof fcb_some_any as [? hh]; specialize (hh fcb); rewrite <-efs; [eapply hh; apply support_fresh; assumption | assumption]].
   Qed.
 
-  Lemma support_empty : support ɛ@{Perm} ≡ ∅.
-  Proof. unfold support; simpl; reflexivity. Qed.
-
-  Definition alpha_rec: Term →ₛ X. refine (λₛ⟦L⟧ t, perm_alpha_rec t ɛ).
+  Definition alpha_rec: Λ →ₛ X. refine (λₛ⟦L⟧ t, perm_alpha_rec t ɛ).
   Proof.
     - repeat intro; apply perm_alpha_rec_respectfull; assumption.
     - intros; apply perm_alpha_rec_supported; rewrite support_empty; set_solver.
   Defined.
 
-  Lemma alpha_rec_respectfull m n : 
-    aeqCof m n → alpha_rec m ≡ alpha_rec n.
+  Lemma alpha_rec_respectfull (m n: Λ) : 
+    m ≡α n → alpha_rec m ≡ alpha_rec n.
   Proof. intros; unfold alpha_rec; simpl; apply perm_alpha_rec_respectfull; assumption. Qed.
 
-  Lemma alpha_rec_var a : 
+  Lemma alpha_rec_var (a: Name) : 
     alpha_rec (Var a) = fvar a.
   Proof. unfold alpha_rec; simpl; rewrite gact_id; auto. Qed.
   
-  Lemma alpha_rec_app (m n: Term):
+  Lemma alpha_rec_app (m n: Λ):
     alpha_rec (App m n) = fapp (alpha_rec m, alpha_rec n).
   Proof. unfold alpha_rec; simpl; reflexivity. Qed.
 
-  Lemma endgame: 
-    ∀ a t, a ∉ L → alpha_rec (Lam a t) ≡ flam [a](alpha_rec t).
+  Lemma alpha_rec_lam (a: Name) (t: Λ): 
+    a ∉ L → alpha_rec (Lam a t) ≡ flam (a, alpha_rec t).
   Proof.
-    intros; unfold alpha_rec; simpl. set (s := fresh _); apply fsupp_equiv.
+    intros; unfold alpha_rec; simpl; rewrite efs; [| set_solver]; set (s := fresh _); apply fsupp_equiv.
     apply name_abstraction_inv; right; assert (HH: s ∉ (L ∪ support flam ∪ support a ∪ support t ∪ support (perm_alpha_rec t) ∪ support ɛ@{Perm})). { apply is_fresh. } split.
-      + apply alpha_class_inv; right; split.
-        * apply not_elem_of_union in HH as [[[[]%not_elem_of_union ?]%not_elem_of_union ?]%not_elem_of_union ?]; set_solver.
+      + apply fresh_nabs; right; split.
+        * apply not_elem_of_union in HH as [[[[]%not_elem_of_union ?]%not_elem_of_union ?]%not_elem_of_union ?]. set_solver.
         * apply fresh_fun_supp.
           -- apply support_fresh; unfold support, fun_supp_support; simpl; apply not_elem_of_union in HH as [[[[]%not_elem_of_union ?]%not_elem_of_union ?]%not_elem_of_union ?]. assumption.
           -- apply support_fresh; unfold support, fun_supp_support; simpl; apply not_elem_of_union in HH as [[[[]%not_elem_of_union ?]%not_elem_of_union ?]%not_elem_of_union ?]. assumption.
@@ -892,80 +814,3 @@ Section RecursionAlpha.
   Qed.
 
 End RecursionAlpha.
-
-(* Section TermLength.
-
-  From Nominal Require Import Instances.Nat.
-  
-  Fixpoint term_length (t: Term): nat :=
-    match t with
-    | Var a => 1
-    | App m n => (term_length m) + (term_length n)
-    | Lam a m => 1 + (term_length m)
-    end.
-
-  Definition length_fvar: Name →ₛ nat.
-  Proof. refine (λₛ⟦∅⟧ n, 1); intros; apply perm_nat. Defined.
-
-  Definition length_fapp: (nat * nat) →ₛ nat.
-  Proof. 
-    refine (λₛ⟦∅⟧ mn, ((fst mn) + (snd mn))%nat).
-    - intros [] [] [H1 H2]; simpl in *; rewrite H1,H2; reflexivity.
-    - intros ? ? ? ? []; simpl; rewrite !perm_nat; reflexivity.
-  Defined.
-
-  (* Instance: Reflexive (≈α). Proof. Admitted. *)
-  Instance: Proper (equiv ==> (≈α)) abs.
-  Proof. repeat intro; unfold equiv,name_abstraction_equiv in *;
-    destruct x as [[x n]]; destruct y as [[y m]]; assumption.
-  Qed.
-
-  Instance:  Proper (equiv ==> equiv) snd.
-  Proof. intros [] [] [? []]; simpl; rewrite !perm_nat in *; assumption. Qed.
-
-  Definition length_flam: [𝔸]nat →ₛ nat.
-  Proof.
-    refine (λₛ⟦∅⟧ (an: [𝔸]nat), (1 + (snd an))%nat).
-    - repeat intro. rewrite H; reflexivity.
-    - intros; rewrite !perm_nat; unfold action, name_abstraction_action; simpl; rewrite !perm_nat;
-      reflexivity.
-  Defined.
-
-  Lemma name_fresh_nat (a: Name) (n: nat): a # n. Proof. Admitted.
-
-  Lemma length_flam_fcb: FCB length_flam.
-  Proof.
-    unfold FCB; eexists; split.
-    - unfold support; simpl; apply not_elem_of_empty.
-    - intros; apply name_fresh_nat.
-  Unshelve.
-    (* we can use any name. Pick some default *)
-    exact Atom.default.
-  Qed.
-
-  Lemma term_lenght_respectfull: ∀ m n, m ≡ n → term_length m = term_length n.
-  Proof. Admitted. 
-
-  Lemma equal a b m: alpha_rec length_fvar length_fapp length_flam (lamFCB := length_flam_fcb) (⟨a,b⟩•m) = alpha_rec length_fvar length_fapp length_flam (lamFCB := length_flam_fcb) m.
-  Proof. Admitted.
-
-  Lemma length_equal:
-    ∀ t, term_length t = alpha_rec length_fvar length_fapp length_flam (lamFCB := length_flam_fcb) t.
-  Proof.
-    apply alpha_ind.
-    - repeat intro; inversion H; subst;
-      erewrite alpha_rec_respectfull, term_lenght_respectfull; eauto; symmetry.
-      + assumption.
-      + econstructor; eassumption.
-    - intros; rewrite alpha_rec_var; simpl; reflexivity.
-    - intros ? ? A B; rewrite alpha_rec_app; simpl in *; rewrite A, B; reflexivity.
-    - pose proof (alpha_rec_lam_exists_abs length_fvar length_fapp length_flam (lamFCB := length_flam_fcb)).
-    exists ∅; intros. simpl.
-      pose proof alpha_rec_lam_exists_abs.
-
-      pose proof (alpha_rec_lam length_fvar length_fapp length_flam (lamFCB := length_flam_fcb) a m).
-      simpl in *. set (c := fresh _) in *.
-      rewrite H1. f_equal.
-    rewrite alpha_rec_lam.
-
-End TermLength. *)
