theories/FreshnessTheorem.v
@@ -1,0 +1,39 @@
+From Nominal Require Import Nominal Fresh NameAbstraction.
+From Nominal.Instances Require Import SupportedFunctions Name.
+
+Section FT.
+
+Context `{Nominal X} (h: Name →ₛ X) (Hp: ∃ a, a # h ∧ a # (h a)).
+  
+Definition freshF: X := h (fresh (support h)).
+
+Lemma freshness_theorem_some_any: (∃ a, a # h ∧ a # (h a)) ↔ (∀ a, a # h → a # (h a)).
+Proof.
+  split; intros HH.
+  - intros a AH; destruct HH as [b [BH1 BH2]]; destruct (decide (a = b)).
+    + subst; assumption.
+    + apply (fresh_equivariant ⟨a,b⟩) in BH2; 
+      rewrite perm_swap_right,fun_equivar,perm_swap_right,fresh_fixpoint in BH2; assumption.
+  - new c fresh h; exists c; split.
+    + apply support_fresh; assumption.
+    + apply HH, support_fresh; assumption.
+Qed.
+
+Theorem freshness_theorem: ∀ a, a # h → (h a) ≡ freshF.
+Proof.
+  intros a AH; unfold freshF; set (a' := fresh _); destruct (decide (a = a')); subst; try reflexivity.
+  rewrite <-(fresh_fixpoint a a' (h a')), fun_equivar,perm_swap_right,fresh_fixpoint.
+    + reflexivity.
+    + assumption.
+    + apply fresh_support_fresh.
+    + apply fresh_fun_supp; [| apply name_neq_fresh_iff]; assumption.
+    + apply freshness_theorem_some_any; [| apply fresh_support_fresh]; apply Hp.
+Qed.
+
+Corollary freshness_theorem_inj: ∀ a b, a # h → b # h → h a ≡ h b.
+Proof. 
+  intros; rewrite !freshness_theorem; try reflexivity; try assumption;
+  destruct H1 as [x ?]; exists x; split; try (apply support_fresh; tauto); tauto.
+Qed.
+
+End FT.
