theories/Instances/Bool.v
@@ -1,0 +1,27 @@
+From Nominal Require Import Nominal SupportedFunctions.
+
+#[export] Instance bool_action: PermAction bool := λ p b, b.
+#[export] Instance bool_equiv: Equiv bool := eq.
+#[export] Instance bool_support: Support bool := λ b, ∅.
+
+#[export] Instance bool_permT: PermT bool.
+Proof.
+    split; unfold equiv,bool_equiv,action,bool_action in *; auto; repeat intro.
+    - typeclasses eauto.
+    - subst; reflexivity.
+Qed.
+
+#[export] Instance bool_nominal: Nominal bool.
+Proof. 
+    split; intros; [apply bool_permT | unfold action,bool_action; reflexivity].
+Qed.
+
+Section Properties.
+    Context `{Nominal X} (f: X →ₛ bool).
+
+    Lemma lol: ∀ p x, (p•f) x = f (- p • x).
+    Proof. unfold equiv,fun_supp_equiv; intros; rewrite fsupp_action.
+        unfold action at 1; unfold bool_action. reflexivity.
+    Qed.
+    
+End Properties.
